src/DY.Lib.SplitPredicate.fst
@@ -1,0 +1,172 @@
+module DY.Lib.SplitPredicate
+
+#set-options "--fuel 1 --ifuel 1"
+
+// Some kind of cheap module functor like ocaml but in F*
+noeq type split_predicate_input_values = {
+  labeled_data_t: Type;
+  label_t: Type;
+  encoded_label_t: Type;
+  raw_data_t: Type;
+
+  decode_labeled_data: labeled_data_t -> GTot (option (encoded_label_t & raw_data_t));
+
+  encode_label: label_t -> encoded_label_t;
+  encode_label_inj: l1:label_t -> l2:label_t -> Lemma
+    (requires encode_label l1 == encode_label l2)
+    (ensures l1 == l2)
+  ;
+}
+
+// Can probably be generalized to handle kdf usage too?
+type global_pred (func:split_predicate_input_values) =
+  func.labeled_data_t -> prop
+type local_pred (func:split_predicate_input_values) =
+  func.raw_data_t -> prop
+
+val has_local_pred: func:split_predicate_input_values -> global_pred func -> func.label_t -> local_pred func -> prop
+let has_local_pred func gpred the_label lpred =
+  forall labeled_data.
+    match func.decode_labeled_data labeled_data with
+    | Some (label, raw_data) ->
+      label == func.encode_label the_label ==> (gpred labeled_data <==> lpred raw_data)
+    | None -> True
+
+val mk_global_pred: func:split_predicate_input_values -> list (func.label_t & local_pred func) -> global_pred func
+let rec mk_global_pred func l labeled_data =
+  match l with
+  | [] -> False
+  | (the_label, lpred)::t ->
+    let cur_prop =
+      match func.decode_labeled_data labeled_data with
+      | Some (label, raw_data) ->
+        label == func.encode_label the_label /\ lpred raw_data
+      | None -> False
+    in
+    cur_prop \/ mk_global_pred func t labeled_data
+
+val mk_global_pred_wrong_label:
+  func:split_predicate_input_values ->
+  the_label:func.label_t -> l:list (func.label_t & local_pred func) -> labeled_data:func.labeled_data_t ->
+  Lemma
+  (requires ~(List.Tot.memP the_label (List.Tot.map fst l)))
+  (ensures (
+    match func.decode_labeled_data labeled_data with
+    | Some (label, raw_data) ->
+      label == func.encode_label the_label ==> ~(mk_global_pred func l labeled_data)
+    | None -> ~(mk_global_pred func l labeled_data)
+  ))
+let rec mk_global_pred_wrong_label func the_label l labeled_data =
+  match l with
+  | [] -> ()
+  | (label, _)::t -> (
+    FStar.Classical.move_requires_2 func.encode_label_inj the_label label;
+    mk_global_pred_wrong_label func the_label t labeled_data
+  )
+
+val disjointP: #a:Type -> list a -> list a -> prop
+let rec disjointP #a l1 l2 =
+  match l1 with
+  | [] -> True
+  | h1::t1 ->
+    ~(List.Tot.memP h1 l2) /\ disjointP t1 l2
+
+val disjointP_cons:
+  #a:Type ->
+  x:a -> l1:list a -> l2:list a ->
+  Lemma
+  (requires disjointP l1 l2 /\ ~(List.Tot.memP x l1))
+  (ensures disjointP l1 (x::l2))
+let rec disjointP_cons #a x l1 l2 =
+  match l1 with
+  | [] -> ()
+  | h1::t1 -> disjointP_cons x t1 l2
+
+val memP_map:
+  #a:Type -> #b:Type ->
+  f:(a -> b) -> l:list a -> x:a ->
+  Lemma
+  (requires List.Tot.memP x l)
+  (ensures List.Tot.memP (f x) (List.Tot.map f l))
+let rec memP_map #a #b f l x =
+  match l with
+  | [] -> ()
+  | h::t ->
+    introduce x =!= h ==> List.Tot.memP (f x) (List.Tot.map f t)
+    with _. memP_map f t x
+
+val mk_global_pred_correct_aux:
+  func:split_predicate_input_values -> gpred:global_pred func -> lpreds1:list (func.label_t & local_pred func) -> lpreds2:list (func.label_t & local_pred func) -> the_label:func.label_t -> lpred:local_pred func ->
+  Lemma
+  (requires
+    (forall labeled_data. (mk_global_pred func lpreds1 labeled_data \/ mk_global_pred func lpreds2 labeled_data) <==> gpred labeled_data) /\
+    List.Tot.no_repeats_p (List.Tot.map fst lpreds1) /\
+    disjointP (List.Tot.map fst lpreds1) (List.Tot.map fst lpreds2) /\
+    List.Tot.memP (the_label, lpred) lpreds1
+  )
+  (ensures has_local_pred func gpred the_label lpred)
+let rec mk_global_pred_correct_aux func gpred lpreds1 lpreds2 the_label lpred =
+  match lpreds1 with
+  | [] -> ()
+  | (h_lab, h_spred)::t -> (
+    eliminate h_lab == the_label \/ h_lab =!= the_label returns _ with _. (
+      introduce forall labeled_data. (
+        match func.decode_labeled_data labeled_data with
+        | Some (label, raw_data) ->
+          label == func.encode_label the_label ==> (gpred labeled_data <==> lpred raw_data)
+        | None -> True
+      ) with (
+        match func.decode_labeled_data labeled_data with
+        | Some (label, raw_data) -> (
+          eliminate label == func.encode_label the_label \/ label =!= func.encode_label the_label returns _ with _. (
+            func.encode_label_inj the_label h_lab;
+            mk_global_pred_wrong_label func the_label t labeled_data;
+            mk_global_pred_wrong_label func the_label lpreds2 labeled_data;
+            FStar.Classical.move_requires_3 memP_map fst t (the_label, lpred)
+          ) and _. ()
+        )
+        | None -> ()
+      )
+    ) and _. (
+      disjointP_cons h_lab (List.Tot.map fst t) (List.Tot.map fst lpreds2);
+      mk_global_pred_correct_aux func gpred t ((h_lab, h_spred)::lpreds2) the_label lpred
+    )
+  )
+
+val disjointP_nil: #a:Type -> l:list a -> Lemma (disjointP l [])
+let rec disjointP_nil #a l =
+  match l with
+  | [] -> ()
+  | _::t -> disjointP_nil t
+
+val mk_global_pred_correct:
+  func:split_predicate_input_values -> lpreds:list (func.label_t & local_pred func) -> the_label:func.label_t -> lpred:local_pred func ->
+  Lemma
+  (requires
+    List.Tot.no_repeats_p (List.Tot.map fst lpreds) /\
+    List.Tot.memP (the_label, lpred) lpreds
+  )
+  (ensures has_local_pred func (mk_global_pred func lpreds) the_label lpred)
+let mk_global_pred_correct func lpreds the_label lpred =
+  disjointP_nil (List.Tot.map fst lpreds);
+  mk_global_pred_correct_aux func (mk_global_pred func lpreds) lpreds [] the_label lpred
+
+val mk_global_pred_eq:
+  func:split_predicate_input_values -> lpreds:list (func.label_t & local_pred func) ->
+  labeled_data:func.labeled_data_t ->
+  Lemma
+  (mk_global_pred func lpreds labeled_data <==> (
+      exists lab lpred raw_data.
+        List.Tot.memP (lab, lpred) lpreds /\
+        lpred raw_data /\
+        func.decode_labeled_data labeled_data == Some (func.encode_label lab, raw_data)
+    )
+  )
+let rec mk_global_pred_eq func lpreds labeled_data =
+  match lpreds with
+  | [] -> ()
+  | (the_label, lpred)::tpreds ->
+    mk_global_pred_eq func tpreds labeled_data;
+    match func.decode_labeled_data labeled_data with
+    | None -> ()
+    | Some (label, raw_data) -> ()
