src/DY.Lib.State.Labeled.fst
@@ -1,0 +1,213 @@
+module DY.Lib.State.Labeled
+
+open Comparse
+open DY.Core.Label
+open DY.Core.Label.Type
+open DY.Core.Trace.Type
+open DY.Core.Trace.Invariant
+open DY.Core.Trace.Manipulation
+open DY.Core.Bytes
+open DY.Core.Bytes.Type
+open DY.Lib.SplitPredicate
+open DY.Lib.Comparse.Glue
+open DY.Lib.Comparse.Parsers
+
+#set-options "--fuel 1 --ifuel 1"
+
+(*** Session predicates ***)
+
+type session (bytes:Type0) {|bytes_like bytes|} = {
+  [@@@ with_parser #bytes ps_string]
+  label: string;
+  content: bytes;
+}
+
+%splice [ps_session] (gen_parser (`session))
+%splice [ps_session_is_well_formed] (gen_is_well_formed_lemma (`session))
+
+instance parseable_serializeable_session (bytes:Type0) {|bytes_like bytes|}: parseable_serializeable bytes (session bytes) = mk_parseable_serializeable (ps_session)
+
+let split_session_pred_func: split_predicate_input_values = {
+  labeled_data_t = trace & principal & nat & bytes;
+  label_t = string;
+  encoded_label_t = string;
+  raw_data_t = trace & principal & nat & bytes;
+
+  decode_labeled_data = (fun (tr, prin, sess_id, sess_content) -> (
+    match parse (session bytes) sess_content with
+    | Some ({label; content}) -> Some (label, (tr, prin, sess_id, content))
+    | None -> None
+  ));
+
+  encode_label = (fun s -> s);
+  encode_label_inj = (fun l1 l2 -> ());
+}
+
+noeq
+type session_pred = {
+  pred: crypto_predicates -> trace -> principal -> nat -> bytes -> prop;
+  pred_later:
+    cpreds:crypto_predicates ->
+    tr1:trace -> tr2:trace ->
+    prin:principal -> sess_id:nat -> content:bytes ->
+    Lemma
+    (requires pred cpreds tr1 prin sess_id content /\ tr1 <$ tr2)
+    (ensures pred cpreds tr2 prin sess_id content)
+  ;
+  pred_knowable:
+    cpreds:crypto_predicates ->
+    tr:trace -> prin:principal -> sess_id:nat -> content:bytes ->
+    Lemma
+    (requires pred cpreds tr prin sess_id content)
+    (ensures is_knowable_by cpreds (principal_state_label prin sess_id) tr content)
+  ;
+}
+
+val session_pred_to_local_pred:
+  crypto_predicates -> session_pred ->
+  local_pred split_session_pred_func
+let session_pred_to_local_pred cpreds sess_pred (tr, prin, sess_id, content) =
+  sess_pred.pred cpreds tr prin sess_id content
+
+val protocol_predicates_to_global_pred: protocol_predicates -> global_pred split_session_pred_func
+let protocol_predicates_to_global_pred preds (tr, prin, sess_id, content) =
+  preds.trace_preds.state_pred tr prin sess_id content
+
+val has_session_pred: preds:protocol_predicates -> string -> session_pred -> prop
+let has_session_pred pr lab spred =
+  has_local_pred split_session_pred_func (protocol_predicates_to_global_pred pr) lab (session_pred_to_local_pred pr.crypto_preds spred)
+
+(*** Global session predicate builder ***)
+
+val label_session_pred_to_label_local_pred: cpreds:crypto_predicates -> string & session_pred -> string & local_pred split_session_pred_func
+let label_session_pred_to_label_local_pred cpreds (label, spred) =
+  (label, session_pred_to_local_pred cpreds spred)
+
+val mk_global_session_pred: cpreds:crypto_predicates -> list (string & session_pred) -> trace -> principal -> nat -> bytes -> prop
+let mk_global_session_pred cpreds l tr prin sess_id content =
+  mk_global_pred split_session_pred_func (List.Tot.map (label_session_pred_to_label_local_pred cpreds) l) (tr, prin, sess_id, content)
+
+val mk_global_session_pred_correct: preds:protocol_predicates -> lpreds:list (string & session_pred) -> lab:string -> spred:session_pred -> Lemma
+  (requires
+    preds.trace_preds.state_pred == mk_global_session_pred preds.crypto_preds lpreds /\
+    List.Tot.no_repeats_p (List.Tot.map fst lpreds) /\
+    List.Tot.memP (lab, spred) lpreds
+  )
+  (ensures has_session_pred preds lab spred)
+let mk_global_session_pred_correct preds lpreds lab spred =
+  memP_map (label_session_pred_to_label_local_pred preds.crypto_preds) lpreds (lab, spred);
+  FStar.Classical.forall_intro_2 (DY.Misc.index_map (label_session_pred_to_label_local_pred preds.crypto_preds));
+  FStar.Classical.forall_intro_2 (DY.Misc.index_map (fst #string #(session_pred)));
+  FStar.Classical.forall_intro_2 (DY.Misc.index_map (fst #string #(local_pred split_session_pred_func)));
+  List.Tot.index_extensionality (List.Tot.map fst lpreds) (List.Tot.map fst (List.Tot.map (label_session_pred_to_label_local_pred preds.crypto_preds) lpreds));
+  mk_global_pred_correct split_session_pred_func (List.Tot.map (label_session_pred_to_label_local_pred preds.crypto_preds) lpreds) lab (session_pred_to_local_pred preds.crypto_preds spred)
+
+val mk_global_session_pred_later:
+  cpreds:crypto_predicates -> lpreds:list (string & session_pred) ->
+  tr1:trace -> tr2:trace -> prin:principal -> sess_id:nat -> content:bytes -> Lemma
+  (requires mk_global_session_pred cpreds lpreds tr1 prin sess_id content /\ tr1 <$ tr2)
+  (ensures mk_global_session_pred cpreds lpreds tr2 prin sess_id content)
+let rec mk_global_session_pred_later cpreds lpreds tr1 tr2 prin sess_id content =
+  match lpreds with
+  | [] -> ()
+  | (_, lpred)::tpreds ->
+    FStar.Classical.move_requires (mk_global_session_pred_later cpreds tpreds tr1 tr2 prin sess_id) content;
+    FStar.Classical.forall_intro (FStar.Classical.move_requires (lpred.pred_later cpreds tr1 tr2 prin sess_id));
+    // Why F*, why???
+    match parse (session bytes) content with
+    | None -> ()
+    | Some _ -> ()
+
+val mk_global_session_pred_knowable:
+  cpreds:crypto_predicates -> lpreds:list (string & session_pred) ->
+  tr:trace -> prin:principal -> sess_id:nat -> full_content:bytes ->
+  Lemma
+  (requires mk_global_session_pred cpreds lpreds tr prin sess_id full_content)
+  (ensures is_knowable_by cpreds (principal_state_label prin sess_id) tr full_content)
+let rec mk_global_session_pred_knowable cpreds lpreds tr prin sess_id full_content =
+  match lpreds with
+  | [] -> ()
+  | (current_label, current_lpred)::tpreds ->
+    FStar.Classical.move_requires (mk_global_session_pred_knowable cpreds tpreds tr prin sess_id) full_content;
+    match parse (session bytes) full_content with
+    | None -> ()
+    | Some ({label; content}) -> (
+      if label = current_label then (
+        introduce current_lpred.pred cpreds tr prin sess_id content ==> is_knowable_by cpreds (principal_state_label prin sess_id) tr full_content
+        with _. (
+          current_lpred.pred_knowable cpreds tr prin sess_id content;
+          serialize_parse_inv_lemma (session bytes) full_content;
+          serialize_wf_lemma (session bytes) (is_knowable_by cpreds (principal_state_label prin sess_id) tr) ({label; content})
+        )
+      ) else ()
+    )
+
+(*** API for labeled sessions ***)
+
+val set_labeled_state: string -> principal -> nat -> bytes -> crypto unit
+let set_labeled_state lab prin sess_id content =
+  let full_content = {
+    label = lab;
+    content;
+  } in
+  let full_content_bytes = serialize (session bytes) full_content in
+  set_state prin sess_id full_content_bytes
+
+val get_labeled_state: string -> principal -> nat -> crypto (option bytes)
+let get_labeled_state lab prin sess_id =
+  let*? full_content_bytes = get_state prin sess_id in
+  match parse (session bytes) full_content_bytes with
+    | None -> return None
+    | Some ({label; content;}) ->
+      if label = lab then return (Some content)
+      else return None
+
+val set_labeled_state_invariant:
+  preds:protocol_predicates ->
+  label:string -> spred:session_pred ->
+  prin:principal -> sess_id:nat -> content:bytes -> tr:trace ->
+  Lemma
+  (requires
+    spred.pred preds.crypto_preds tr prin sess_id content /\
+    trace_invariant preds tr /\
+    has_session_pred preds label spred
+  )
+  (ensures (
+    let ((), tr_out) = set_labeled_state label prin sess_id content tr in
+    trace_invariant preds tr_out
+  ))
+  [SMTPat (set_labeled_state label prin sess_id content tr);
+   SMTPat (trace_invariant preds tr);
+   SMTPat (has_session_pred preds label spred)]
+let set_labeled_state_invariant preds lab spred prin sess_id content tr =
+  assert_norm (forall tr prin sess_id session. protocol_predicates_to_global_pred preds (tr, prin, sess_id, session) <==> preds.trace_preds.state_pred tr prin sess_id session);
+  let full_content = {
+    label = lab;
+    content;
+  } in
+  parse_serialize_inv_lemma #bytes (session bytes) full_content
+
+val get_labeled_state_invariant:
+  preds:protocol_predicates ->
+  label:string -> spred:session_pred ->
+  prin:principal -> sess_id:nat -> tr:trace ->
+  Lemma
+  (requires
+    trace_invariant preds tr /\
+    has_session_pred preds label spred
+  )
+  (ensures (
+    let (opt_content, tr_out) = get_labeled_state label prin sess_id tr in
+    tr == tr_out /\ (
+      match opt_content with
+      | None -> True
+      | Some content -> (
+        spred.pred preds.crypto_preds tr prin sess_id content
+      )
+    )
+  ))
+  [SMTPat (get_labeled_state label prin sess_id tr);
+   SMTPat (trace_invariant preds tr);
+   SMTPat (has_session_pred preds label spred)]
+let get_labeled_state_invariant preds lab spred prin sess_id tr =
+  assert_norm (forall tr prin sess_id session. protocol_predicates_to_global_pred preds (tr, prin, sess_id, session) <==> preds.trace_preds.state_pred tr prin sess_id session)
