src/DY.Misc.fst
@@ -1,0 +1,11 @@
+module DY.Misc
+
+open FStar.List.Tot
+
+val index_map: #a:Type -> #b:Type -> f:(a -> b) -> l:list a -> i:nat{i < List.Tot.length l} -> Lemma (
+  index (map f l) i == f (index l i)
+)
+let rec index_map #a #b f l i =
+  let h::t = l in
+  if i = 0 then ()
+  else index_map f t (i-1)
